src/PlutusIR/Semantics/SemanticEquivalence/Contextual.v
@@ -23,12 +23,12 @@ Definition contextually_approximate
   (Δ ,, Γ |-+ e  : T) /\
   (Δ ,, Γ |-+ e' : T) /\
   forall (C : context),
-    ([] ,, [] |-C C : (Δ ,, Γ ▷ T) ↝ ty_unit) ->
-      context_apply C e ==> val_unit ->
-      context_apply C e' ==> val_unit
+    ([] ,, [] |- C : (Δ, Γ, T) ↪ ty_unit) ->
+      context_fill C e ==> val_unit ->
+      context_fill C e' ==> val_unit
 .
 
-Notation "Δ ',,' Γ '|-' e1 ⪯-ctx e2 ':' T" := (contextually_approximate e1 e2 Δ Γ T)
+Notation "Δ ',,' Γ '|-' e1 ≤-ctx e2 ':' T" := (contextually_approximate e1 e2 Δ Γ T)
   ( at level 101
   , e1 at level 0
   , e2 at level 0
@@ -38,25 +38,11 @@ Notation "Δ ',,' Γ '|-' e1 ⪯-ctx e2 ':' T" := (contextually_approximate e1 e
 Definition contextually_equivalent
   (e e' : term) Δ Γ T
   :=
-  (Δ ,, Γ |- e ⪯-ctx e' : T )
-  /\ (Δ ,, Γ |- e'⪯-ctx e  : T)
+  (Δ ,, Γ |- e ≤-ctx e' : T )
+  /\ (Δ ,, Γ |- e'≤-ctx e  : T)
   .
 
-Notation "Δ ',,' Γ '|-' e1 ≃-ctx e2 ':' T" := (contextually_equivalent e1 e2 Δ Γ T)
-  ( at level 101
-  , e1 at level 0
-  , e2 at level 0
-  , T at level 0
-  , no associativity).
-
-(* ciu = Closed Instantiations of Use *)
-
-Definition ciu_equivalent e e' T :=
-  ([],, [] |-+ e  : T)  /\
-  ([],, [] |-+ e' : T) /\
-  ((e ⇓) <-> (e' ⇓)).
-
-Notation "|- e1 ≃-ciu e2 ':' T" := (ciu_equivalent e1 e2 T)
+Notation "Δ ',,' Γ '|-' e1 =ctx e2 ':' T" := (contextually_equivalent e1 e2 Δ Γ T)
   ( at level 101
   , e1 at level 0
   , e2 at level 0
@@ -67,7 +53,7 @@ Section contextually_approximate_lemmas.
 
   Lemma contextually_approximate_reflexive : forall Δ Γ e T,
   Δ ,, Γ |-+ e : T ->
-  Δ ,, Γ |- e ⪯-ctx e : T.
+  Δ ,, Γ |- e ≤-ctx e : T.
   Proof.
     unfold contextually_approximate.
     intros.
@@ -75,9 +61,9 @@ Section contextually_approximate_lemmas.
   Qed.
 
   Lemma contextually_approximate_transitive : forall Δ Γ e1 e2 e3 T,
-    Δ ,, Γ |- e1 ⪯-ctx e2 : T ->
-    Δ ,, Γ |- e2 ⪯-ctx e3 : T ->
-    Δ ,, Γ |- e1 ⪯-ctx e3 : T.
+    Δ ,, Γ |- e1 ≤-ctx e2 : T ->
+    Δ ,, Γ |- e2 ≤-ctx e3 : T ->
+    Δ ,, Γ |- e1 ≤-ctx e3 : T.
   Proof with eauto.
     unfold contextually_approximate.
     intros.
@@ -86,17 +72,17 @@ Section contextually_approximate_lemmas.
   Qed.
 
   Lemma contextually_approximate_antisymmetric : forall Δ Γ e1 e2 T,
-    Δ ,, Γ |- e1 ⪯-ctx e2 : T ->
-    Δ ,, Γ |- e2 ⪯-ctx e1 : T ->
-    Δ ,, Γ |- e1 ≃-ctx e2 : T.
+    Δ ,, Γ |- e1 ≤-ctx e2 : T ->
+    Δ ,, Γ |- e2 ≤-ctx e1 : T ->
+    Δ ,, Γ |- e1 =ctx e2 : T.
   Proof.
     unfold contextually_equivalent.
     eauto.
   Qed.
 
-  Notation "⪯-ctx-refl" := (contextually_approximate_reflexive).
-  Notation "⪯-ctx-trans" := (contextually_approximate_transitive).
-  Notation "⪯-ctx-antisym" := (contextually_approximate_antisymmetric).
+  Notation "≤-ctx-refl" := (contextually_approximate_reflexive).
+  Notation "≤-ctx-trans" := (contextually_approximate_transitive).
+  Notation "≤-ctx-antisym" := (contextually_approximate_antisymmetric).
 
 End contextually_approximate_lemmas.
 
@@ -104,32 +90,32 @@ Section contextually_equivalent_props.
 
   Lemma contextually_equivalent_reflexive : forall Δ Γ e T,
   Δ ,, Γ |-+ e : T ->
-  Δ ,, Γ |- e ≃-ctx e : T.
+  Δ ,, Γ |- e =ctx e : T.
   Proof.
     unfold contextually_equivalent.
     auto using contextually_approximate_reflexive.
   Qed.
 
   Lemma contextually_equivalent_transitive : forall Δ Γ e1 e2 e3 T,
-    Δ ,, Γ |- e1 ≃-ctx e2 : T ->
-    Δ ,, Γ |- e2 ≃-ctx e3 : T ->
-    Δ ,, Γ |- e1 ≃-ctx e3 : T.
+    Δ ,, Γ |- e1 =ctx e2 : T ->
+    Δ ,, Γ |- e2 =ctx e3 : T ->
+    Δ ,, Γ |- e1 =ctx e3 : T.
   Proof.
     unfold contextually_equivalent.
     intuition; eauto using contextually_approximate_transitive.
   Qed.
 
   Lemma contextually_equivalent_symmetric : forall Δ Γ e1 e2 T,
-    Δ ,, Γ |- e1 ≃-ctx e2 : T ->
-    Δ ,, Γ |- e2 ≃-ctx e1 : T.
+    Δ ,, Γ |- e1 =ctx e2 : T ->
+    Δ ,, Γ |- e2 =ctx e1 : T.
   Proof.
     unfold contextually_equivalent.
     intuition.
   Qed.
 
 
-  Notation "≃-ctx-refl" := (contextually_equivalent_reflexive).
-  Notation "≃-ctx-trans" := (contextually_equivalent_transitive).
-  Notation "≃-ctx-sym" := (contextually_equivalent_symmetric).
+  Notation "=ctx-refl" := (contextually_equivalent_reflexive).
+  Notation "=ctx-trans" := (contextually_equivalent_transitive).
+  Notation "=ctx-sym" := (contextually_equivalent_symmetric).
 
 End contextually_equivalent_props.
